make Steel.PCMReference.witness, recall ghost

pulse/ulib/experimental/Steel.PCMReference.fst
@@ -77,15 +77,15 @@ let gather r v0 v1 =
                  (fun _ -> ());
   gather' r v0 v1
 
-val witness' (#a:Type) (#pcm:pcm a)
+val witness' (#inames: _) (#a:Type) (#pcm:pcm a)
             (r:ref a pcm)
             (fact:stable_property pcm)
             (v:erased a)
             (_:fact_valid_compat fact v)
-  : SteelT unit (pts_to r v)
+  : SteelGhostT unit inames (pts_to r v)
                 (fun _ -> to_vprop Mem.(pts_to r v `star` pure (witnessed r fact)))
 
-let witness' r fact v _ = as_action (Steel.Memory.witness FStar.Set.empty r fact v ())
+let witness' #inames r fact v _ = as_atomic_action_ghost (Steel.Memory.witness inames r fact v ())
 
 let witness r fact v s =
   witness' r fact v s;
@@ -94,16 +94,16 @@ let witness r fact v s =
                  (fun _ -> ());
   elim_pure (witnessed r fact)
 
-val recall' (#a:Type u#1) (#pcm:pcm a) (fact:property a)
+val recall' (#inames: _) (#a:Type u#1) (#pcm:pcm a) (fact:property a)
            (r:ref a pcm)
            (v:erased a)
-  : SteelT (v1:erased a{compatible pcm v v1})
+  : SteelGhostT (v1:erased a{compatible pcm v v1}) inames
            (to_vprop Mem.(pts_to r v `star` pure (witnessed r fact)))
            (fun v1 -> to_vprop Mem.(pts_to r v `star` pure (fact v1)))
 
-let recall' #a #pcm fact r v = as_action (Steel.Memory.recall #a #pcm #fact FStar.Set.empty r v)
+let recall' #inames #a #pcm fact r v = as_atomic_action_ghost (Steel.Memory.recall #a #pcm #fact inames r v)
 
-let recall #a #pcm fact r v =
+let recall #inames #a #pcm fact r v =
   intro_pure (witnessed r fact);
   rewrite_slprop (pts_to r v `star` pure (witnessed r fact))
                  (to_vprop Mem.(pts_to r v `star` pure (witnessed r fact)))
